PREFIX : <https://linked.data.gov.au/dataset/gnaf/code/geocodeReliability/> 
PREFIX cs: <https://linked.data.gov.au/dataset/gnaf/code/geocodeReliability> 
PREFIX dcterms: <http://purl.org/dc/terms/> 
PREFIX status: <http://def.isotc211.org/iso19135/-1/2015/CoreModel/code/RE_ItemStatus/> 
PREFIX rdfs: <http://www.w3.org/2000/01/rdf-schema#> 
PREFIX sdo: <https://schema.org/> 
PREFIX skos: <http://www.w3.org/2004/02/skos/core#> 
PREFIX reg: <http://purl.org/linked-data/registry#> 
PREFIX xsd: <http://www.w3.org/2001/XMLSchema#> 

:1 a skos:Concept ;
    dcterms:identifier "1"^^xsd:token ;
    reg:status status:submitted ;
    rdfs:isDefinedBy cs: ;
    skos:definition "Geocode Accuracy Recorded To Appropriate Surveying Standard"@en ;
    skos:inScheme cs: ;
    skos:prefLabel "Surveying Standard"@en ;
    skos:topConceptOf cs: .

:2 a skos:Concept ;
    dcterms:identifier "2"^^xsd:token ;
    reg:status status:submitted ;
    rdfs:isDefinedBy cs: ;
    skos:definition "Geocode Accuracy Sufficient To Place Centroid Within Address Site Boundary Or Access Point"@en ;
    skos:inScheme cs: ;
    skos:prefLabel "Within Address Site Boundary Or Access Point"@en ;
    skos:topConceptOf cs: .

:3 a skos:Concept ;
    dcterms:identifier "3"^^xsd:token ;
    reg:status status:submitted ;
    rdfs:isDefinedBy cs: ;
    skos:definition "Geocode Accuracy Sufficient To Place Centroid Near (Or Possibly Within) Address Site Boundary"@en ;
    skos:inScheme cs: ;
    skos:prefLabel "Near (Or Possibly Within) Address Site Boundary"@en ;
    skos:topConceptOf cs: .

:4 a skos:Concept ;
    dcterms:identifier "4"^^xsd:token ;
    reg:status status:submitted ;
    rdfs:isDefinedBy cs: ;
    skos:definition "Geocode Accuracy Sufficient To Associate Address Site With A Unique Road Feature"@en ;
    skos:inScheme cs: ;
    skos:prefLabel "Unique Road Feature"@en ;
    skos:topConceptOf cs: .

:5 a skos:Concept ;
    dcterms:identifier "5"^^xsd:token ;
    reg:status status:submitted ;
    rdfs:isDefinedBy cs: ;
    skos:definition "Geocode Accuracy Sufficient To Associate Address Site With A Unique Locality Or Neighbourhood"@en ;
    skos:inScheme cs: ;
    skos:prefLabel "Unique Locality Or Neighbourhood"@en ;
    skos:topConceptOf cs: .

:6 a skos:Concept ;
    dcterms:identifier "6"^^xsd:token ;
    reg:status status:submitted ;
    rdfs:isDefinedBy cs: ;
    skos:definition "Geocode Accuracy Sufficient To Associate Address Site With A Unique Region"@en ;
    skos:inScheme cs: ;
    skos:prefLabel "Unique Region"@en ;
    skos:topConceptOf cs: .

cs: a skos:ConceptScheme ;
    dcterms:created "2018-02-10"^^xsd:date ;
    dcterms:identifier "geocodeReliability"^^xsd:token ;
    dcterms:modified "2022-06-01"^^xsd:date ;
    dcterms:provenance "Automatically created from the G-NAF codelists"@en ;
    skos:definition "Description of the geocode reliability code"@en ;
    skos:hasTopConcept :1,
        :2,
        :3,
        :4,
        :5,
        :6 ;
    skos:prefLabel "Geocode Reliability"@en ;
    sdo:creator <https://linked.data.gov.au/org/ga> ;
    sdo:publisher <https://linked.data.gov.au/org/icsm> .

