PREFIX cs: <https://linked.data.gov.au/def/fsdf/ground-relations>
PREFIX dcterms: <http://purl.org/dc/terms/>
PREFIX fsdf: <https://linked.data.gov.au/def/fsdf/>
PREFIX ground: <https://linked.data.gov.au/def/fsdf/ground-relations/>
PREFIX owl: <http://www.w3.org/2002/07/owl#>
PREFIX rdfs: <http://www.w3.org/2000/01/rdf-schema#>
PREFIX reg: <http://purl.org/linked-data/registry#>
PREFIX skos: <http://www.w3.org/2004/02/skos/core#>
PREFIX status: <http://def.isotc211.org/iso19135/-1/2015/CoreModel/code/RE_ItemStatus/>
PREFIX xsd: <http://www.w3.org/2001/XMLSchema#>

ground:aboveAndBelowGround
    a
        skos:Concept ,
        fsdf:GroundRelation ;
    dcterms:identifier "aboveAndBelowGround"^^xsd:token ;
    reg:status status:submitted ;
    rdfs:isDefinedBy cs: ;
    skos:broader
        ground:aboveGround ,
        ground:belowGround ;
    skos:definition "The Feature is both above - on or over - and below - under - the earth's surface"@en ;
    skos:inScheme cs: ;
    skos:prefLabel "Above and Below Ground"@en ;
    skos:topConceptOf cs: ;
.

ground:atGround
    a
        skos:Concept ,
        fsdf:GroundRelation ;
    dcterms:identifier "atGround"^^xsd:token ;
    reg:status status:submitted ;
    rdfs:isDefinedBy cs: ;
    skos:definition "The Feature in the place of the earth's surface"@en ;
    skos:inScheme cs: ;
    skos:prefLabel "At Ground"@en ;
    skos:topConceptOf cs: ;
.

ground:unknown
    a
        skos:Concept ,
        fsdf:GroundRelation ;
    dcterms:identifier "unknown"^^xsd:token ;
    reg:status status:submitted ;
    rdfs:isDefinedBy cs: ;
    skos:definition "The Feature's relation to the 'earth's surface is not known"@en ;
    skos:inScheme cs: ;
    skos:prefLabel "Unknown"@en ;
    skos:topConceptOf cs: ;
.

ground:aboveGround
    a
        skos:Concept ,
        fsdf:GroundRelation ;
    dcterms:identifier "aboveGround"^^xsd:token ;
    reg:status status:submitted ;
    rdfs:isDefinedBy cs: ;
    skos:definition "The Feature is entirely above - on or over - the earth's surface"@en ;
    skos:inScheme cs: ;
    skos:prefLabel "Above Ground"@en ;
    skos:topConceptOf cs: ;
.

ground:belowGround
    a
        skos:Concept ,
        fsdf:GroundRelation ;
    dcterms:identifier "belowGround"^^xsd:token ;
    reg:status status:submitted ;
    rdfs:isDefinedBy cs: ;
    skos:definition "The Feature is entirely below - or under - the earth's surface"@en ;
    skos:inScheme cs: ;
    skos:prefLabel "Below Ground"@en ;
    skos:topConceptOf cs: ;
.

cs:
    a
        owl:Ontology ,
        skos:ConceptScheme ;
    dcterms:created "2021-06-08"^^xsd:date ;
    dcterms:creator <https://linked.data.gov.au/org/ga> ;
    dcterms:identifier "ground-relations"^^xsd:token ;
    dcterms:license <http://purl.org/NET/rdflicense/cc-by4.0> ;
    dcterms:modified "2021-06-08"^^xsd:date ;
    dcterms:provenance "Created for the Loc-I DR Project"@en ;
    dcterms:publisher <https://linked.data.gov.au/org/icsm> ;
    owl:versionInfo "1.0"^^xsd:string ;
    reg:status status:submitted ;
    skos:definition "This vocabulary lists relations of geospatial Feature to the earth's surface"@en ;
    skos:hasTopConcept
        ground:aboveGround ,
        ground:atGround ,
        ground:belowGround ,
        ground:unknown ;
    skos:prefLabel "FSDF Ground Relations" ;
.

